Make linking even more general

theories/language/wp_link.v
@@ -199,36 +199,6 @@ Definition spec_union (p1 p2 : program_specification) : program_specification :=
 Definition spec_inters (p1 p2 : program_specification) : program_specification := 
   λ s vv Φ, (p1 s vv Φ ∧ p2 s vv Φ)%I.
 
-(*
-Lemma link_progs T1 T2 (p1 : gmap string (Λ.(func))) F s':
-    ⌜s' ∉ dom p1⌝
- -∗ □(T2 |- p1 :: T1)
- -∗ □(∀ vv Φ, T2 s' vv Φ -∗ WP (of_class _ (ExprCall s' vv)) @ (mkPe ∅ T1); ⊤ {{v, Φ v}})
- -∗ (λ s vv Φ, T2 s vv Φ ∧ ⌜s <> s'⌝) |- (<[s':=F]> p1) :: (spec_union T1 (λ s vv Φ, ⌜s = s'⌝ ∧ T2 s vv Φ)).
-Proof.
-  iIntros (Hdom) "#Hp1 #Hp2".
-  iAssert (∀ Φ e, ((WP e @ (mkPe p1 T2); ⊤ {{v,Φ v}}) ∨ (WP e @ (mkPe ∅ T1); ⊤ {{v,Φ v}})) -∗
-      WP e @ (mkPe ((<[s':=F]> p1)) ((λ s vv Φ, T2 s vv Φ ∧ ⌜s <> s'⌝))); ⊤ {{v,Φ v}})%I as "Hsol";
-  first (iLöb as "IH"; iIntros (Φ e) "[HWP|HWP]").
-  3: {
-    iIntros (s vv Φ) "[Hspec|(-> & Hspec)]".
-    - iApply "Hsol". iLeft. iApply ("Hp1" with "Hspec").
-    - iApply "Hsol". iRight. iApply ("Hp2" with "Hspec"). }
-  1-2: rewrite !wp_unfold /wp_pre /=;
-       iIntros "%σ %ns Hσ"; iSpecialize ("HWP" $! σ ns with "Hσ");
-       iMod "HWP" as "[(%x & -> & Hσ & H)|[(%s & %vv & %K & -> & %H2 & >(%Ξ & Hσ & HT & H3))|(%HH & H3)]]".
-  - iModIntro. iLeft. iExists x. iFrame. done.
-  - destruct (decide (s=s')) as [<-|Hne].
-    + 
-
-  2: {
-    iIntros (s vv Φ) "[Hspec|(-> & Hspec)]".
-    - iApply "Hsol". iLeft. iApply ("Hp1" with "Hspec").
-    - iApply "Hsol". iRight. iApply ("Hp2" with "Hspec").
-    }
-  
-    *)
-
 Lemma reducible_no_threads_mono p1 p2 e σ : p1 ⊆ p2 -> reducible_no_threads p1 e σ -> reducible_no_threads p2 e σ.
 Proof.
   intros Hsub (e2 & σ2 & (K & e1' & e2' & -> & -> & H)%prim_step_inv).
@@ -241,219 +211,232 @@ Proof.
     eapply lookup_weaken; done. 
   - eapply head_step_no_call; done. 
 Qed.
+Notation prog := (gmap string (Λ.(func))).
 
-Definition can_link T1 T2 T3 Tres (p1 p2 p3 : gmap string (Λ.(func))) :iProp Σ := 
-   ⌜dom p1 ## dom p2⌝
- ∗ □(∀ s vv Φ, T3 s vv Φ -∗ ⌜s ∉ dom p1⌝ ∗ ⌜s ∉ dom p2⌝)
- ∗ □(∀ s vv Φ, Tres s vv Φ -∗ (spec_union T1 T2) s vv Φ)
- ∗ □(spec_union T2 T3 |- p1 :: T1)
- ∗ □(spec_union T1 T3 |- p2 :: T2)
- ∗ ⌜p3 = (union_with (λ _ _ : func Λ, None) p1 p2)⌝.
 
-Lemma wp_link_execs T1 T2 T3 Tres (p1 p2 p3 : gmap string (Λ.(func))) :
-  can_link T1 T2 T3 Tres p1 p2 p3
- -∗ ∀ e Φ,
-    WP e @ mkPe p1 (spec_union T2 T3); ⊤ {{ v, Φ v }} ∨ WP e @ mkPe p2 (spec_union T1 T3); ⊤ {{ v, Φ v }} -∗
-    WP e @ mkPe p3 (T3); ⊤ {{ v, Φ v }}.
+Class can_link (T1 T2 Taxiom Tres : program_specification) (p1 p2 p3 : prog) : Prop := {
+  p1_p2_disjoint : dom p1 ## dom p2;
+  Tres_is_union : ⊢ (∀ s vv Φ, Tres s vv Φ -∗ (spec_union T1 T2) s vv Φ)%I;
+  Taxiom_is_axiomatic : ⊢ (∀ s vv Φ, Taxiom s vv Φ -∗ ⌜s ∉ dom p3⌝)%I;
+  p1_satisfies_T1 : ⊢ (spec_union T2 Taxiom |- p1 :: T1)%I;
+  p2_satisfies_T2 : ⊢ (spec_union T1 Taxiom |- p2 :: T2)%I;
+  p3_is_union : p3 = (union_with (λ _ _ : func Λ, None) p1 p2);
+}.
+
+Definition pairwise {X} (A:list X) (T : X -> X -> Prop) :=
+  forall i j, i <> j -> match (nth_error A i, nth_error A j) with
+      (Some a, Some b) => T a b
+     | _ => True end.
+
+Definition spec_union_list (P : list program_specification) : program_specification := 
+  λ s vv Φ, (∃ i, match nth_error P i with Some pp => pp s vv Φ | _ => ⌜False⌝ end)%I.
+Definition spec_union_list_except k (P : list program_specification) : program_specification := 
+  λ s vv Φ, (∃ i, ⌜i <> k⌝ ∗ match nth_error P i with Some pp => pp s vv Φ | _ => ⌜False⌝ end)%I.
+
+Fixpoint union_map_list (P : list prog) : prog := match P with
+  nil => ∅
+ | x::xr => union_with (λ _ _ : func Λ, None) x (union_map_list xr)
+end.
+
+Lemma pairwise_subset {X} H (a : list X) x : pairwise (x::a) H -> pairwise a H.
 Proof.
-  iIntros "(%Hdis & #HT3 & _ & #Hp1 & #Hp2 & ->)".
-  iLöb as "IHe". iIntros (e Φ).
-  rewrite !wp_unfold /wp_pre /=.
-  iIntros "[H|H] %σ %ns Hσ".
-  - iSpecialize ("H" $! σ ns with "Hσ").
-    iMod "H".
-    iDestruct "H" as "[(%x & -> & Hσ & H)|[(%s' & %vv' & %K & %HeqK & %H2 & >(%Ξ & Hσ & [HT|HT] & H3))|(%HH & H3)]]".
-    * iModIntro. iLeft. iExists _. iFrame. iPureIntro. done.
-    * destruct (p2 !! s') as [v|] eqn:Heqp2.
-      ++ iRight. iRight.
-         iPoseProof ("Hp2" $! _ _ _ with "HT") as "(%HNone & HT)".
-         rewrite wp_unfold /wp_pre /=.
-         iSpecialize ("HT" $! σ ns with "Hσ").
-         iMod "HT" as "[(%x & %Heqx & Hσ & H)|[(%s'2 & %vv'2 & %K'2 & %HeqK2 & %H''2 & >(%Ξ' & Hσ & HT' & H3'))|(%HH2&H3')]]".
-         -- exfalso. apply of_class_inj in Heqx. congruence.
-         -- exfalso. assert (K'2 = empty_ectx) as ->. 
-            2: { rewrite fill_empty in HeqK2. apply of_class_inj in HeqK2. assert (s'2 = s') as -> by congruence; congruence. }
-            destruct (fill_class K'2 (of_class Λ (ExprCall s'2 vv'2))) as [H1|[x Hx]].
-            { eexists. rewrite <- HeqK2. by rewrite to_of_class. }
-            { done. }
-            { exfalso. unfold to_val in Hx. rewrite to_of_class in Hx; congruence. }
-         -- destruct HH2 as (e' & σ' & (KK & e1' & e2' & Heq2 & -> & Hstep)%prim_step_inv).
-            destruct (fill_class KK e1') as [->|[x Hx]].
-            { eexists. rewrite <- Heq2. by rewrite to_of_class. }
-            2: { apply val_head_stuck in Hstep. congruence. }
-            rewrite ! fill_empty in Heq2. subst e1'.
-            apply call_head_step in Hstep.
-            destruct Hstep as (Fn & Heqp2' & He2' & -> & _ ).
-            iModIntro. iSplit; first iPureIntro.
-            { do 2 eexists. rewrite HeqK. econstructor; first done. 1:done.
-              apply call_head_step. exists Fn. repeat split; try done.
-              rewrite lookup_union_with. rewrite Heqp2'. rewrite H2. done. }
-            subst e. iIntros (? ? (e'2 & -> & (Fn3 & Heqp3' & He3' & -> & _ )%call_head_step)%head_reducible_prim_step_ctx).
-            2: { do 3 eexists.
-                 apply call_head_step. exists Fn. repeat split; try done.
-                 rewrite lookup_union_with. rewrite Heqp2'. rewrite H2. done. }
-            rewrite lookup_union_with in Heqp3'. rewrite Heqp2' in Heqp3'. rewrite H2 in Heqp3'.
-            cbn in Heqp3'. iSpecialize ("H3'" $! σ e2').
-            assert (prim_step p2 (of_class Λ (ExprCall s' vv')) σ e2' σ []) as Hstep2.
-            { apply head_prim_step. apply call_head_step. eexists; repeat split; done. }
-            iSpecialize ("H3'" $! Hstep2). iMod "H3'". iModIntro. iNext.
-            iMod "H3'" as "(? & H3')". iModIntro. iFrame.
-            iApply wp_bind. iApply (wp_wand with "[H3']").
-            { iApply "IHe"; iRight. assert (e'2 = e2') as -> by congruence. iApply "H3'". }
-            iIntros (r) "Hr". iSpecialize ("H3" $! r with "Hr"). iApply "IHe". iLeft. done.
-      ++ iRight. iLeft. iModIntro.
-         rewrite HeqK. do 3 iExists _. iSplitR; first done.
-         iSplitR.
-         { iPureIntro. rewrite lookup_union_with. rewrite H2. rewrite Heqp2. done. }
-         iDestruct ("Hp2" with "HT") as "(%HNone2 & _)". congruence.
-    * iRight. iLeft. iModIntro. do 3 iExists _; iSplitR; first done.
-      rewrite lookup_union_with. rewrite H2. destruct (p2!!s') eqn:Heq.
-      1: { iDestruct ("HT3" with "HT") as "(%Hne1 & %Hne2)".
-           exfalso. apply Hne2. apply elem_of_dom. by eexists. }
-      cbn. iSplitR; first done. iModIntro. iExists Ξ. iFrame. iNext.
-      iIntros (r) "Hr". iSpecialize ("H3" with "Hr"). iApply "IHe". iLeft. done.
-    * iModIntro. iRight. iRight.
-      iSplitR.
-      { iPureIntro. eapply reducible_no_threads_mono; last done.
-        intros k. rewrite lookup_union_with. destruct (p1 !! k) as [f1|] eqn:Heq1;
-        destruct (p2 !! k) as [f2|] eqn:Heq2.
-        2-4: done. 
-        cbn. apply elem_of_disjoint in Hdis. eapply Hdis; apply elem_of_dom; eexists; done. }
-      iIntros (σ' e' Hstep%prim_step_inv).
-      iSpecialize ("H3" $! σ' e').
-      destruct Hstep as (K & e1' & e2' & -> & -> & H).
-      assert (prim_step p1 (fill K e1') σ (fill K e2') σ' []) as Hstep.
-      { econstructor. 1-2:done. destruct (to_class e1') as [[]|] eqn:Heq.
-        - exfalso. eapply val_head_step. apply of_to_class in Heq. erewrite Heq. done.
-        - apply of_to_class in Heq. subst e1'.
-          destruct HH as (? & σ'2 & (e2'' & -> & (K2 & eK1 & eK2 & Heq1 & -> & HHstep)%prim_step_inv)%fill_step_inv).
-          2: unfold to_val; by rewrite to_of_class.
-          assert (K2 = empty_ectx) as ->.
-          1: { destruct (fill_class' K2 eK1) as [|[vv Hvv]].
-               1: eexists; rewrite <- Heq1; by rewrite to_of_class.
-               1: done.
-               exfalso. apply of_to_class in Hvv. subst eK1. eapply val_head_step. done. }
-          rewrite fill_empty in Heq1. subst eK1. apply call_head_step in H, HHstep.
-          destruct H as (FN1 & HFN1 &Happy1 & -> & _).
-          destruct HHstep as (FN2 & HFN2 &Happy2 & -> & _).
-          rewrite lookup_union_with in HFN1. rewrite HFN2 in HFN1. destruct (p2 !! fn_name); cbn in *; try congruence.
-          apply call_head_step. exists FN2. repeat split; try congruence.
-        - by eapply head_step_no_call. }
-      iDestruct ("H3" $! Hstep) as ">H3". iModIntro. iNext.
-      iMod "H3" as "(Hσ & HWP)". iModIntro. iFrame. iApply "IHe". by iLeft.
-
-
-
-
-  - iSpecialize ("H" $! σ ns with "Hσ").
-    iMod "H".
-    iDestruct "H" as "[(%x & -> & Hσ & H)|[(%s' & %vv' & %K & %HeqK & %H2 & >(%Ξ & Hσ & [HT|HT] & H3))|(%HH & H3)]]".
-    * iModIntro. iLeft. iExists _. iFrame. iPureIntro. done.
-    * destruct (p1 !! s') as [v|] eqn:Heqp2.
-      ++ iRight. iRight.
-         iPoseProof ("Hp1" $! _ _ _ with "HT") as "(_ & HT)".
-         rewrite wp_unfold /wp_pre /=.
-         iSpecialize ("HT" $! σ ns with "Hσ").
-         iMod "HT" as "[(%x & %Heqx & Hσ & H)|[(%s'2 & %vv'2 & %K'2 & %HeqK2 & %H''2 & >(%Ξ' & Hσ & HT' & H3'))|(%HH2&H3')]]".
-         -- exfalso. apply of_class_inj in Heqx. congruence.
-         -- exfalso. assert (K'2 = empty_ectx) as ->. 
-            2: { rewrite fill_empty in HeqK2. apply of_class_inj in HeqK2. assert (s'2 = s') as -> by congruence; congruence. }
-            destruct (fill_class K'2 (of_class Λ (ExprCall s'2 vv'2))) as [H1|[x Hx]].
-            { eexists. rewrite <- HeqK2. by rewrite to_of_class. }
-            { done. }
-            { exfalso. unfold to_val in Hx. rewrite to_of_class in Hx; congruence. }
-         -- destruct HH2 as (e' & σ' & (KK & e1' & e2' & Heq2 & -> & Hstep)%prim_step_inv).
-            destruct (fill_class KK e1') as [->|[x Hx]].
-            { eexists. rewrite <- Heq2. by rewrite to_of_class. }
-            2: { apply val_head_stuck in Hstep. congruence. }
-            rewrite ! fill_empty in Heq2. subst e1'.
-            apply call_head_step in Hstep.
-            destruct Hstep as (Fn & Heqp2' & He2' & -> & _ ).
-            iModIntro. iSplit; first iPureIntro.
-            { do 2 eexists. rewrite HeqK. econstructor; first done. 1:done.
-              apply call_head_step. exists Fn. repeat split; try done.
-              rewrite lookup_union_with. rewrite Heqp2'. rewrite H2. done. }
-            subst e. iIntros (? ? (e'2 & -> & (Fn3 & Heqp3' & He3' & -> & _ )%call_head_step)%head_reducible_prim_step_ctx).
-            2: { do 3 eexists.
-                 apply call_head_step. exists Fn. repeat split; try done.
-                 rewrite lookup_union_with. rewrite Heqp2'. rewrite H2. done. }
-            rewrite lookup_union_with in Heqp3'. rewrite Heqp2' in Heqp3'. rewrite H2 in Heqp3'.
-            cbn in Heqp3'. iSpecialize ("H3'" $! σ e2').
-            assert (prim_step p1 (of_class Λ (ExprCall s' vv')) σ e2' σ []) as Hstep2.
-            { apply head_prim_step. apply call_head_step. eexists; repeat split; done. }
-            iSpecialize ("H3'" $! Hstep2). iMod "H3'". iModIntro. iNext.
-            iMod "H3'" as "(? & H3')". iModIntro. iFrame.
-            iApply wp_bind. iApply (wp_wand with "[H3']").
-            { iApply "IHe"; iLeft. assert (e'2 = e2') as -> by congruence. iApply "H3'". }
-            iIntros (r) "Hr". iSpecialize ("H3" $! r with "Hr"). iApply "IHe". iRight. done.
-      ++ iRight. iLeft. iModIntro.
-         rewrite HeqK. do 3 iExists _. iSplitR; first done.
-         iSplitR.
-         { iPureIntro. rewrite lookup_union_with. rewrite H2. rewrite Heqp2. done. }
-         iDestruct ("Hp1" with "HT") as "(%HNone2 & _)". congruence.
-    * iRight. iLeft. iModIntro. do 3 iExists _; iSplitR; first done.
-      rewrite lookup_union_with. rewrite H2. destruct (p1!!s') eqn:Heq.
-      1: { iDestruct ("HT3" with "HT") as "(%Hne1 & %Hne2)".
-           exfalso. apply Hne1. apply elem_of_dom. by eexists. }
-      cbn. iSplitR; first done. iModIntro. iExists Ξ. iFrame. iNext.
-      iIntros (r) "Hr". iSpecialize ("H3" with "Hr"). iApply "IHe". iRight. done.
-    * iModIntro. iRight. iRight.
-      iSplitR.
-      { iPureIntro. eapply reducible_no_threads_mono; last done.
-        intros k. rewrite lookup_union_with. destruct (p1 !! k) as [f1|] eqn:Heq1;
-        destruct (p2 !! k) as [f2|] eqn:Heq2.
-        2-4: done. 
-        cbn. apply elem_of_disjoint in Hdis. eapply Hdis; apply elem_of_dom; eexists; done. }
-      iIntros (σ' e' Hstep%prim_step_inv).
-      iSpecialize ("H3" $! σ' e').
-      destruct Hstep as (K & e1' & e2' & -> & -> & H).
-      assert (prim_step p2 (fill K e1') σ (fill K e2') σ' []) as Hstep.
-      { econstructor. 1-2:done. destruct (to_class e1') as [[]|] eqn:Heq.
-        - exfalso. eapply val_head_step. apply of_to_class in Heq. erewrite Heq. done.
-        - apply of_to_class in Heq. subst e1'.
-          destruct HH as (? & σ'2 & (e2'' & -> & (K2 & eK1 & eK2 & Heq1 & -> & HHstep)%prim_step_inv)%fill_step_inv).
-          2: unfold to_val; by rewrite to_of_class.
-          assert (K2 = empty_ectx) as ->.
-          1: { destruct (fill_class' K2 eK1) as [|[vv Hvv]].
-               1: eexists; rewrite <- Heq1; by rewrite to_of_class.
-               1: done.
-               exfalso. apply of_to_class in Hvv. subst eK1. eapply val_head_step. done. }
-          rewrite fill_empty in Heq1. subst eK1. apply call_head_step in H, HHstep.
-          destruct H as (FN1 & HFN1 &Happy1 & -> & _).
-          destruct HHstep as (FN2 & HFN2 &Happy2 & -> & _).
-          rewrite lookup_union_with in HFN1. rewrite HFN2 in HFN1. destruct (p1 !! fn_name); cbn in *; try congruence.
-          apply call_head_step. exists FN2. repeat split; try congruence.
-        - by eapply head_step_no_call. }
-      iDestruct ("H3" $! Hstep) as ">H3". iModIntro. iNext.
-      iMod "H3" as "(Hσ & HWP)". iModIntro. iFrame. iApply "IHe". by iRight.
+  intros HH i j Hne.
+  specialize (HH (S i) (S j)). cbn in HH.
+  apply HH. congruence.
 Qed.
 
-Lemma wp_link_progs T1 T2 T3 Tres (p1 p2 p3 : gmap string (Λ.(func))) :
-    can_link T1 T2 T3 Tres p1 p2 p3
- -∗ T3 |- p3 :: Tres.
+Lemma union_map_list_spec x y (P:list prog) : 
+  (pairwise P (fun p1 p2 => dom p1 ## dom p2)) -> 
+  ((union_map_list P) !! x = Some y <-> ∃ k, In k P ∧ k !! x = Some y).
 Proof.
-  iIntros "(%Hdis & #HT3 & #Hres & #Hp1 & #Hp2 & ->)".
-  iIntros (s vv Φ) "H". iDestruct ("Hres" with "H") as "[H|H]".
-  - iPoseProof ("Hp1" with "H") as "(%HNone & HH)".
-    destruct (p2 !! s) eqn:Heq.
-    * exfalso. pose proof (elem_of_disjoint (dom p1) (dom p2)) as [Hdis2 _].
-      destruct (p1 !! s) eqn:Heqq; try congruence.
-      eapply Hdis2; first done.
-      all: apply elem_of_dom; eexists; try done. 
-    * iSplitR.
-      -- iPureIntro. rewrite lookup_union_with. 
-         rewrite Heq. destruct (p1 !! s); cbn; congruence.
-      -- iApply (wp_link_execs with "[HT3 Hp2] [HH]"); last by iLeft. unfold can_link; repeat iSplit; (try by iPureIntro); done.
-  - iDestruct ("Hp2" with "H") as "(%HNone & HH)".
-    destruct (p1 !! s) eqn:Heq.
-    * exfalso. pose proof (elem_of_disjoint (dom p1) (dom p2)) as [Hdis2 _].
-      destruct (p2 !! s) eqn:Heqq; try congruence.
-      eapply Hdis2; first done.
-      all: apply elem_of_dom; eexists; try done. 
-    * iSplitR.
-      -- iPureIntro. rewrite lookup_union_with. 
-         rewrite Heq. destruct (p2 !! s); cbn; congruence.
-      -- iApply (wp_link_execs with "[HT3 Hp2] [HH]"); last by iRight. unfold can_link; repeat iSplit; (try by iPureIntro); done.
+  intros Hdis.
+  revert x y.
+  induction P; intros x y; first split; cbn.
+  - rewrite lookup_empty. intros H; congruence.
+  - intros (? & [] & ?).
+  - rewrite lookup_union_with.
+    destruct (a !! x) as [va|] eqn:Hva;
+    destruct (union_map_list P !! x) as [vP|] eqn:HvP; cbn; split; try congruence.
+    + intros _. apply IHP in HvP; last by eapply pairwise_subset.
+      destruct HvP as (k & (pos & Hpos)%In_nth_error & Heq).
+      specialize (Hdis 0 (S pos)); cbn in Hdis. rewrite Hpos in Hdis.
+      exfalso. assert (0 ≠ S pos) as Hne by lia. specialize (Hdis Hne).
+      rewrite  elem_of_disjoint in Hdis. eapply Hdis.
+      all: by eapply elem_of_dom_2.
+    + injection 1; intros ->. exists a; repeat split; by try left.
+    + intros (k & [-> | Hk] & Heq); first congruence.
+      exfalso. assert (∃ k : prog, In k P ∧ k !! x = Some y) as H by by exists k.
+      apply IHP in H; first congruence. by eapply pairwise_subset.
+    + apply IHP in HvP; last by eapply pairwise_subset.
+      destruct HvP as (k & ? & ?).
+      injection 1; intros ->. exists k; repeat split; eauto.
+    + intros (k & [-> | Hk] & Heq); first congruence.
+      assert (∃ k : prog, In k P ∧ k !! x = Some y) as H by by exists k.
+      apply IHP in H; last by eapply pairwise_subset. congruence.
+    + intros (k & [-> | Hk] & Heq); first congruence.
+      assert (∃ k : prog, In k P ∧ k !! x = Some y) as H by by exists k.
+      apply IHP in H; last by eapply pairwise_subset. congruence.
+Qed.
+
+Lemma union_map_subset A p : 
+  (pairwise A (fun p1 p2 => dom p1 ## dom p2)) -> p ∈ A → p ⊆ union_map_list A.
+Proof.
+  intros Hdis H. apply map_subseteq_spec.
+  intros i x Hin.
+  apply union_map_list_spec; first done.
+  exists p. split; eauto. by apply elem_of_list_In.
+Qed.
+
+Record can_link_all 
+    (Taxiom Tres : program_specification) (pres : prog)
+    (A : list (prod program_specification prog)) := {
+  all_disjoint : pairwise (map snd A) (fun p1 p2 => dom p1 ## dom p2);
+  Tres_is_big_union : ⊢ (∀ s vv Φ, Tres s vv Φ -∗ (spec_union_list (map fst A)) s vv Φ)%I;
+  Taxiom_is_axiomatic_all : ⊢ (∀ s vv Φ, Taxiom s vv Φ -∗ ⌜s ∉ dom pres⌝)%I;
+  pres_is_union : pres = union_map_list (map snd A);
+  one_spec := fun i => spec_union (spec_union_list_except i (map fst A)) Taxiom;
+  all_satisfy_spec : ∀ i, match (nth_error A i) with None => True |
+      Some (Ti, pi) =>  ⊢ (one_spec i |- pi :: Ti)%I end
+}.
+
+Lemma can_link_can_link_all Taxiom Tres pres T1 T2 p1 p2 : can_link T1 T2 Taxiom Tres p1 p2 pres
+  -> can_link_all Taxiom Tres pres [(T1,p1); (T2,p2)].
+Proof.
+  intros [H1 H2 H3 H4 H5 H6]; split; cbn.
+  - intros [|[|[|i]]] [|[|[|j]]] H; cbn; easy.
+  - iIntros (s vv Φ) "Hres". iPoseProof H2 as "H2".
+    iDestruct ("H2" $! s vv Φ with "Hres") as "[H2'|H2']".
+    + iExists 0; cbn; done.
+    + iExists 1; cbn; done.
+  - done.
+  - rewrite H6. apply map_eq. intros i. rewrite ! lookup_union_with. rewrite lookup_empty.
+    destruct (p1 !! i), (p2 !! i); done.
+  - intros [|[|[|i]]]; cbn; try done.
+    all: iIntros (s vv Φ) "Hres"; cbn.
+    1: iPoseProof H4 as "H"; iSpecialize ("H" $! s vv Φ with "Hres").
+    2: iPoseProof H5 as "H"; iSpecialize ("H" $! s vv Φ with "Hres").
+    all: iDestruct "H" as "[$ HWP]".
+    all: iApply wp_pe_mono; last iApply "HWP".
+    all: split; first done; cbn; intros s' vv' Φ'; iIntros (Hnot) "[H|H]".
+    2,4: by iRight. all: iLeft.
+    1: iExists 1. 2: iExists 0.
+    all: iSplitR; first done. all: done.
+Qed.
+
+Lemma wp_link_execs Taxiom Tres (pres : gmap string (Λ.(func))) A :
+  can_link_all Taxiom Tres pres A
+  -> ⊢ ∀ e Φ i, match (nth_error A i) with None => ⌜False⌝ | 
+          Some (Ti, pi) => WP e @ mkPe pi
+          (spec_union (spec_union_list_except i (map fst A)) Taxiom); ⊤ {{ v, Φ v }} end
+     -∗ WP e @ mkPe pres (Taxiom); ⊤ {{ v, Φ v }}.
+Proof.
+  intros [Hdis HTres Haxiom -> one_spec' Hsatis].
+  iLöb as "IHe". iIntros (e Φ i).
+  destruct (nth_error A i) as [[Ti pi]|] eqn:Heq; last (iIntros "%H"; done).
+  rewrite !wp_unfold /wp_pre /=.
+  iIntros "H %σ %ns Hσ".
+  - iSpecialize ("H" $! σ ns with "Hσ").
+    iMod "H".
+    iDestruct "H" as "[(%x & -> & Hσ & H)|[(%s' & %vv' & %K & %HeqK & %H2 & >(%Ξ & Hσ & [HT|HT] & H3))|(%HH & H3)]]".
+    * iModIntro. iLeft. iExists _. iFrame. iPureIntro. done.
+    * iDestruct "HT" as "(%kidx & %Hknei & HT)". rewrite nth_error_map.
+      destruct (nth_error A kidx) as [[Tc pc]|] eqn:Heqk; cbn; last iPure "HT" as [].
+      specialize (Hsatis kidx). rewrite Heqk in Hsatis.
+      iPoseProof (Hsatis) as "Hsatis".
+      iDestruct ("Hsatis" $! s' vv' Ξ with "HT")as "(%HNone & HT)".
+      rewrite wp_unfold /wp_pre /=.
+      iSpecialize ("HT" $! σ ns with "Hσ").
+      iMod "HT" as "[(%x & %Heqx & Hσ & H)|[(%s'2 & %vv'2 & %K'2 & %HeqK2 & %H''2 & >(%Ξ' & Hσ & HT' & H3'))|(%HH2&H3')]]".
+      -- exfalso. apply of_class_inj in Heqx. congruence.
+      -- exfalso. assert (K'2 = empty_ectx) as ->. 
+         2: { rewrite fill_empty in HeqK2. apply of_class_inj in HeqK2. assert (s'2 = s') as -> by congruence; congruence. }
+         destruct (fill_class K'2 (of_class Λ (ExprCall s'2 vv'2))) as [H1|[x Hx]].
+         { eexists. rewrite <- HeqK2. by rewrite to_of_class. }
+        { done. }
+          { exfalso. unfold to_val in Hx. rewrite to_of_class in Hx; congruence. }
+     -- destruct HH2 as (e' & σ' & (KK & e1' & e2' & Heq2 & -> & Hstep)%prim_step_inv).
+          destruct (fill_class KK e1') as [->|[x Hx]].
+         { eexists. rewrite <- Heq2. by rewrite to_of_class. }
+         2: { apply val_head_stuck in Hstep. congruence. }
+         rewrite ! fill_empty in Heq2. subst e1'.
+         apply call_head_step in Hstep.
+         destruct Hstep as (Fn & Heqp2' & He2' & -> & _ ). iRight. iRight.
+         assert (union_map_list (map snd A) !! s' = Some Fn) as Heqs'.
+         { apply union_map_list_spec; first done. exists pc; repeat split; try done.
+           apply in_map_iff. exists ((Tc,pc)); repeat split. by eapply nth_error_In. }
+         iModIntro. iSplit; first iPureIntro.
+         { do 2 eexists. rewrite HeqK. econstructor; first done. 1:done.
+           apply call_head_step. exists Fn. repeat split; try done. }
+         subst e. iIntros (? ? (e'2 & -> & (Fn3 & Heqp3' & He3' & -> & _ )%call_head_step)%head_reducible_prim_step_ctx).
+         2: { do 3 eexists.
+              apply call_head_step. exists Fn. repeat split; try done. }
+         rewrite Heqs' in Heqp3'. assert (e'2 = e2') as -> by congruence.
+         iSpecialize ("H3'" $! σ e2').
+         assert (prim_step pc (of_class Λ (ExprCall s' vv')) σ e2' σ []) as Hstep2.
+         { apply head_prim_step. apply call_head_step. eexists; repeat split; done. }
+         iSpecialize ("H3'" $! Hstep2). iMod "H3'". iModIntro. iNext.
+         iMod "H3'" as "(? & H3')". iModIntro. iFrame.
+         iApply wp_bind. iApply (wp_wand with "[H3']").
+         { iApply ("IHe" $! _ _ kidx). rewrite Heqk. iApply "H3'". }
+         iIntros (r) "Hr". iSpecialize ("H3" $! r with "Hr"). iApply ("IHe" $! _ _ i). rewrite Heq. done.
+    * iRight. iLeft. iModIntro. do 3 iExists _; iSplitR; first done.
+      destruct (union_map_list (map snd A) !! s') as [v|] eqn:Heqv.
+      { iExFalso. iDestruct (Haxiom $! s' vv' Ξ with "HT") as "%Hfalse". exfalso.
+        apply Hfalse. eapply elem_of_dom_2. done. }
+      cbn. iSplitR; first done. iModIntro. iExists Ξ. iFrame. iNext.
+      iIntros (r) "Hr". iSpecialize ("H3" with "Hr"). iApply ("IHe" $! _ _ i). by rewrite Heq.
+    * iModIntro. iRight. iRight.
+      iSplitR.
+      { iPureIntro. eapply reducible_no_threads_mono; last done.
+        apply union_map_subset; first done. apply elem_of_list_In.
+        apply in_map_iff. exists ((Ti, pi)); split; eauto.
+        by eapply nth_error_In. }
+      iIntros (σ' e' Hstep%prim_step_inv).
+      iSpecialize ("H3" $! σ' e').
+      destruct Hstep as (K & e1' & e2' & -> & -> & H).
+      assert (prim_step pi (fill K e1') σ (fill K e2') σ' []) as Hstep.
+      { econstructor. 1-2:done. destruct (to_class e1') as [[]|] eqn:Heqe1.
+        - exfalso. eapply val_head_step. apply of_to_class in Heqe1. erewrite Heqe1. done.
+        - apply of_to_class in Heqe1. subst e1'.
+          destruct HH as (? & σ'2 & (e2'' & -> & (K2 & eK1 & eK2 & Heq1 & -> & HHstep)%prim_step_inv)%fill_step_inv).
+          2: unfold to_val; by rewrite to_of_class.
+          assert (K2 = empty_ectx) as ->.
+          1: { destruct (fill_class' K2 eK1) as [|[vv Hvv]].
+               1: eexists; rewrite <- Heq1; by rewrite to_of_class.
+               1: done.
+               exfalso. apply of_to_class in Hvv. subst eK1. eapply val_head_step. done. }
+          rewrite fill_empty in Heq1. subst eK1. apply call_head_step in H, HHstep.
+          destruct H as (FN1 & HFN1 &Happy1 & -> & _).
+          destruct HHstep as (FN2 & HFN2 &Happy2 & -> & _).
+          apply union_map_list_spec in HFN1; last done. destruct HFN1 as (? & [[TT kk] [<- (kki & Hkki)%In_nth_error]]%in_map_iff & HFN1).
+          cbn in HFN1. destruct (decide (kki = i)) as [-> | Hcontr].
+          1: apply call_head_step; exists FN2; repeat split; try congruence.
+          exfalso. specialize (Hdis kki i Hcontr). rewrite ! nth_error_map in Hdis.
+          rewrite Hkki in Hdis. rewrite Heq in Hdis. cbn in Hdis. rewrite elem_of_disjoint in Hdis.
+          eapply Hdis; eapply elem_of_dom_2; done.
+        - by eapply head_step_no_call. }
+      iDestruct ("H3" $! Hstep) as ">H3". iModIntro. iNext.
+      iMod "H3" as "(Hσ & HWP)". iModIntro. iFrame. iApply ("IHe" $! _ _ i). rewrite Heq. done.
+Qed.
+
+Lemma wp_link_progs Taxiom Tres (pres : gmap string (Λ.(func))) A :
+  can_link_all Taxiom Tres pres A
+ -> ⊢ Taxiom |- pres :: Tres.
+Proof.
+  intros [Hdis HTres Haxiom -> one_spec' Hsatis].
+  iIntros (s vv Φ) "H". iPoseProof HTres as "HTres".
+    iDestruct ("HTres" with "H") as "[%x Hx]".
+    erewrite nth_error_map.
+    destruct (nth_error A x) as [[Ti pi]|] eqn:Heq; last by iExFalso. cbn.
+    specialize (Hsatis x) as Hsatis2.
+    rewrite Heq in Hsatis2. iDestruct (Hsatis2 $! s vv Φ with "Hx") as "[%Hx1 Hx2]".
+    destruct (union_map_list (map snd A) !! s) eqn:Hl2.
+  - iSplitR; first done. unshelve iApply (wp_link_execs _ _ _ _ _ $! _ _ x). 3: by split. rewrite Heq. done.
+  - exfalso. destruct (pi !! s) as [f|] eqn:Heqpi; try congruence.
+    assert (∃ k, In k ((map snd A)) ∧ k !! s = Some f) as HH.
+    + exists pi; repeat split; try done. apply in_map_iff. exists (Ti,pi).
+      repeat split; try done. eapply nth_error_In. done.
+    + apply union_map_list_spec in HH; try congruence. done.
 Qed.
 
 
